@prefix : <http://purl.org/sco/ns#> .
@prefix cc: <https://creativecommons.org/ns#> .
@prefix dc: <http://purl.org/dc/elements/1.1/> .
@prefix wn: <https://wordnet-rdf.princeton.edu/ontology#> .
@prefix dbc: <http://dbpedia.org/page/Category:> .
@prefix dbo: <http://dbpedia.org/ontology/> .
@prefix dbr: <http://dbpedia.org/resource/> .
@prefix dct: <http://purl.org/dc/terms/> .
@prefix ebg: <http://data.businessgraph.io/ontology#> .
@prefix m4i: <http://w3id.org/nfdi4ing/metadata4ing#> .
@prefix mod: <https://w3id.org/mod#> .
@prefix org: <http://www.w3.org/ns/org#> .
@prefix owl: <http://www.w3.org/2002/07/owl#> .
@prefix rdf: <http://www.w3.org/1999/02/22-rdf-syntax-ns#> .
@prefix rov: <http://www.w3.org/ns/regorg#> .
@prefix sco: <http://purl.org/sco/ns#> .
@prefix xml: <http://www.w3.org/XML/1998/namespace> .
@prefix xsd: <http://www.w3.org/2001/XMLSchema#> .
@prefix bibo: <http://purl.org/ontology/bibo/> .
@prefix foaf: <http://xmlns.com/foaf/0.1/> .
@prefix rdfs: <http://www.w3.org/2000/01/rdf-schema#> .
@prefix skos: <http://www.w3.org/2004/02/skos/core#> .
@prefix vann: <http://purl.org/vocab/vann/> .
@prefix schema: <http://schema.org/> .
@base <http://purl.org/sco/ns#> .

<http://purl.org/sco/ns#> rdf:type owl:Ontology ;
                           owl:versionIRI <http://purl.org/sco/ns#> ;
                           dct:created "2024"^^xsd:gYear ;
                           dct:creator [ schema:affiliation [ foaf:homepage <https://www.scs.fraunhofer.de/de/ueber-uns/organisation/data-spaces-and-iot-solutions.html> ;
                                                              foaf:name "Data Spaces and IoT Solutions"
                                                            ] ;
                                         rdfs:seeAlso <https://renedorsch.solidweb.org/#me> ;
                                         foaf:homepage <https://orcid.org/0000-0001-6857-7314> ;
                                         foaf:name "Rene Dorsch"
                                       ] ;
                           dct:description "This is the Service Capability (SCO). SCO is a light-weight, application ontology for the translation of legacy IoT devices to the W3C Web of Things. SCO contributes to the automatic generation of Thing Descriptions for modeling the key components necessary for a W3C Web of Things Thing Description.  "@en ;
                           dct:issued "2024-01-14"^^xsd:date ;
                           dct:license <https://creativecommons.org/licenses/by-sa/4.0/> ;
                           dct:publisher <https://renedorsch.solidweb.org/#me> ;
                           dct:title "Service Capability Ontology"@en ;
                           bibo:doi <https://doi.org/10.5281/zenodo.7447958> ;
                           vann:preferredNamespacePrefix "sco" ;
                           vann:preferredNamespaceURI "http://purl.org/sco/ns#" ;
                           owl:versionInfo 1.0 ;
                           foaf:depiction <http://purl.org/sco/schema_diagram> ;
                           cc:license <https://creativecommons.org/licenses/by-sa/4.0/> ;
                           mod:acronym "SCO" ;
                           mod:competencyQuestion <http://purl.org/sco/repository/cq> ;
                           mod:hasSyntax <http://www.w3.org/ns/formats/Turtle> .

#################################################################
#    Annotation properties
#################################################################

###  http://purl.org/dc/terms/created
dct:created rdf:type owl:AnnotationProperty .


###  http://purl.org/dc/terms/creator
dct:creator rdf:type owl:AnnotationProperty .


###  http://purl.org/dc/terms/description
dct:description rdf:type owl:AnnotationProperty .


###  http://purl.org/dc/terms/issued
dct:issued rdf:type owl:AnnotationProperty .


###  http://purl.org/dc/terms/license
dct:license rdf:type owl:AnnotationProperty .


###  http://purl.org/dc/terms/publisher
dct:publisher rdf:type owl:AnnotationProperty .


###  http://purl.org/dc/terms/title
dct:title rdf:type owl:AnnotationProperty .


###  http://purl.org/ontology/bibo/doi
bibo:doi rdf:type owl:AnnotationProperty .


###  http://purl.org/vocab/vann/preferredNamespacePrefix
vann:preferredNamespacePrefix rdf:type owl:AnnotationProperty .


###  http://purl.org/vocab/vann/preferredNamespaceURI
vann:preferredNamespaceURI rdf:type owl:AnnotationProperty .


###  http://schema.org/affiliation
schema:affiliation rdf:type owl:AnnotationProperty .


###  http://xmlns.com/foaf/0.1/depiction
foaf:depiction rdf:type owl:AnnotationProperty .


###  http://xmlns.com/foaf/0.1/homepage
foaf:homepage rdf:type owl:AnnotationProperty .


###  http://xmlns.com/foaf/0.1/name
foaf:name rdf:type owl:AnnotationProperty .


###  https://creativecommons.org/ns#license
cc:license rdf:type owl:AnnotationProperty .


###  https://w3id.org/mod#acronym
mod:acronym rdf:type owl:AnnotationProperty .


###  https://w3id.org/mod#competencyQuestion
mod:competencyQuestion rdf:type owl:AnnotationProperty .


###  https://w3id.org/mod#hasSyntax
mod:hasSyntax rdf:type owl:AnnotationProperty .


#################################################################
#    Object Properties
#################################################################

###  http://purl.org/sco/ns#dataModelOf
sco:dataModelOf rdf:type owl:ObjectProperty ;
                owl:inverseOf sco:hasDataModel ;
                rdfs:domain sco:DataModel ;
                rdfs:range sco:ServiceCapability ;
                rdfs:comment "Represents the connection of data model to a specific service capability." ;
                rdfs:label "is datamodel of" .


###  http://purl.org/sco/ns#decodingRuleOf
sco:decodingRuleOf rdf:type owl:ObjectProperty ;
                   rdfs:subPropertyOf sco:transformationRuleOf ;
                   owl:inverseOf sco:hasDecodingRule ;
                   rdfs:domain sco:TransformationRule ;
                   rdfs:range sco:DataModel ;
                   rdfs:comment "Is the decoding rule (a specail type of transformation rule) for some data model." ;
                   rdfs:label "is decoding rule of" .


###  http://purl.org/sco/ns#encodingRuleOf
sco:encodingRuleOf rdf:type owl:ObjectProperty ;
                   rdfs:subPropertyOf sco:transformationRuleOf ;
                   owl:inverseOf sco:hasEncodingRule ;
                   rdfs:domain sco:TransformationRule ;
                   rdfs:range sco:DataModel ;
                   rdfs:comment "Is the encoding rule (a specail type of transformation rule) for some data model." ;
                   rdfs:label "is encoding rule of" .


###  http://purl.org/sco/ns#hasDataModel
sco:hasDataModel rdf:type owl:ObjectProperty ,
                          owl:FunctionalProperty ;
                 rdfs:domain sco:ServiceCapability ;
                 rdfs:range sco:DataModel ;
                 rdfs:comment "References to the data model of a service capability of a device." ;
                 rdfs:label "has datamodel" .


###  http://purl.org/sco/ns#hasDecodingRule
sco:hasDecodingRule rdf:type owl:ObjectProperty ;
                    rdfs:subPropertyOf sco:hasTransformationRule ;
                    rdfs:domain sco:DataModel ;
                    rdfs:range sco:TransformationRule ;
                    rdfs:comment "Identifies the transformation rule as a decoding rule, to decode some data provided by the device." ;
                    rdfs:label "has decoding rule" .


###  http://purl.org/sco/ns#hasEncodingRule
sco:hasEncodingRule rdf:type owl:ObjectProperty ;
                    rdfs:subPropertyOf sco:hasTransformationRule ;
                    rdfs:domain sco:DataModel ;
                    rdfs:range sco:TransformationRule ;
                    rdfs:comment "Identifies the transformation rule as a encoding rule, to encode some data provided for the device." ;
                    rdfs:label "has encoding rule" .


###  http://purl.org/sco/ns#hasInputFormat
sco:hasInputFormat rdf:type owl:ObjectProperty ;
                   owl:inverseOf sco:inputFormatOf ;
                   rdf:type owl:FunctionalProperty ;
                   rdfs:domain sco:DataModel ;
                   rdfs:range sco:Format ;
                   rdfs:comment "Defines the expected inputformat for some data of a service capability." ;
                   rdfs:label "has inputformat" .


###  http://purl.org/sco/ns#hasInteraction
sco:hasInteraction rdf:type owl:ObjectProperty ;
                   owl:inverseOf sco:interactionOf ;
                   rdfs:domain sco:ServiceCapability ;
                   rdfs:range sco:ServiceInteraction ;
                   rdfs:comment "Indicates the interaction provided by a service capability through a specific service interaction method." ;
                   rdfs:label "has interaction" .


###  http://purl.org/sco/ns#hasManufacturer
sco:hasManufacturer rdf:type owl:ObjectProperty ;
                    owl:inverseOf sco:manufacturerOf ;
                    rdfs:domain sco:Device ;
                    rdfs:range owl:Thing .


###  http://purl.org/sco/ns#hasOutputFormat
sco:hasOutputFormat rdf:type owl:ObjectProperty ;
                    owl:inverseOf sco:outputFormatOf ;
                    rdf:type owl:FunctionalProperty ;
                    rdfs:domain sco:DataModel ;
                    rdfs:range sco:Format ;
                    rdfs:comment "Defines the expected outputformat for some data of a service capability." ;
                    rdfs:label "has outputformat" .


###  http://purl.org/sco/ns#hasProtocolStack
sco:hasProtocolStack rdf:type owl:ObjectProperty ;
                     owl:inverseOf sco:protocolStackOf ;
                     rdfs:domain sco:ServiceInteraction ;
                     rdfs:range sco:ProtocolStack ;
                     rdfs:comment "Refers to the set of network protocols used by a device or service." ;
                     rdfs:label "has protocolstack" .


###  http://purl.org/sco/ns#hasServiceCapability
sco:hasServiceCapability rdf:type owl:ObjectProperty ;
                         owl:inverseOf sco:serviceCapabilityOf ;
                         rdfs:domain sco:Device ;
                         rdfs:range sco:ServiceCapability ;
                         rdfs:comment "Highlights the relation between the service capability and the device." ;
                         rdfs:label "has servicecapability" .


###  http://purl.org/sco/ns#hasTransformationRule
sco:hasTransformationRule rdf:type owl:ObjectProperty ;
                          owl:inverseOf sco:transformationRuleOf ;
                          rdfs:domain sco:DataModel ;
                          rdfs:range sco:TransformationRule ;
                          rdfs:comment "The rule used on some data provided through the data model." ;
                          rdfs:label "has transformation rule" .


###  http://purl.org/sco/ns#hasUnit
sco:hasUnit rdf:type owl:ObjectProperty ;
            owl:inverseOf sco:unitOf ;
            rdf:type owl:FunctionalProperty ;
            rdfs:domain sco:DataModel ;
            rdfs:range owl:Thing ;
            rdfs:comment "Links the unit of some data provided by the device to the data model." ;
            rdfs:label "has unit" .


###  http://purl.org/sco/ns#inputFormatOf
sco:inputFormatOf rdf:type owl:ObjectProperty ;
                  rdfs:domain sco:Format ;
                  rdfs:range sco:DataModel ;
                  rdfs:comment "Is the expected inputformat from the device after executing the optionally transformation function." ;
                  rdfs:label "is inputformat of" .


###  http://purl.org/sco/ns#interactionOf
sco:interactionOf rdf:type owl:ObjectProperty ;
                  rdfs:domain sco:ServiceInteraction ;
                  rdfs:range sco:ServiceCapability ;
                  rdfs:comment "References to a service interaction that is part of a specific service capability." ;
                  rdfs:label "is interaction of" .


###  http://purl.org/sco/ns#manufacturerOf
sco:manufacturerOf rdf:type owl:ObjectProperty ;
                   rdfs:subPropertyOf owl:topObjectProperty ;
                   rdfs:domain owl:Thing ;
                   rdfs:range sco:Device ;
                   rdfs:comment "Links the manufacturer to a specifc device." ;
                   rdfs:label "is manufacturer of" .


###  http://purl.org/sco/ns#outputFormatOf
sco:outputFormatOf rdf:type owl:ObjectProperty ;
                   rdfs:domain sco:Format ;
                   rdfs:range sco:DataModel ;
                   rdfs:comment "Is the expected outputformat from the device after executing the optionally transformation function." ;
                   rdfs:label "is output format of" .


###  http://purl.org/sco/ns#protocolStackOf
sco:protocolStackOf rdf:type owl:ObjectProperty ;
                    rdfs:domain sco:ProtocolStack ;
                    rdfs:range sco:ServiceInteraction ;
                    rdfs:comment "Is the protocol stack used for some interaction with a service capability." ;
                    rdfs:label "is protocolstack of" .


###  http://purl.org/sco/ns#serviceCapabilityOf
sco:serviceCapabilityOf rdf:type owl:ObjectProperty ;
                        rdfs:domain sco:ServiceCapability ;
                        rdfs:range sco:Device ;
                        rdfs:comment "Is the service capability of a device." ;
                        rdfs:label "is servicecapability of" .


###  http://purl.org/sco/ns#transformationRuleOf
sco:transformationRuleOf rdf:type owl:ObjectProperty ;
                         rdfs:domain sco:TransformationRule ;
                         rdfs:range sco:DataModel ;
                         rdfs:comment "Is the transformation rule for some data model." ;
                         rdfs:label "is transformationrule of" .


###  http://purl.org/sco/ns#unitOf
sco:unitOf rdf:type owl:ObjectProperty ;
           rdfs:domain owl:Thing ;
           rdfs:range sco:DataModel ;
           rdfs:comment "A unit of a data model." ;
           rdfs:label "is unit of" .


#################################################################
#    Data properties
#################################################################

###  http://purl.org/sco/ns#hasAddress
sco:hasAddress rdf:type owl:DatatypeProperty ,
                        owl:FunctionalProperty ;
               rdfs:domain sco:ServiceInteraction ;
               rdfs:range xsd:string ;
               rdfs:comment "The address of a service capability to interact with it. E.g. a href for HTTP." ;
               rdfs:label "has Address" .


###  http://purl.org/sco/ns#hasManufacturer
sco:hasManufacturer rdf:type owl:DatatypeProperty .


###  http://purl.org/sco/ns#hasName
sco:hasName rdf:type owl:DatatypeProperty ;
            rdfs:domain [ rdf:type owl:Class ;
                          owl:unionOf ( sco:Device
                                        sco:ServiceCapability
                                      )
                        ] ;
            rdfs:range xsd:string ;
            rdfs:comment "The name of a device. Often a device provides a prefered name (e.g. Bluetooth LE or ZigBee)." ;
            rdfs:label "has Name" .


#################################################################
#    Classes
#################################################################

###  http://purl.org/sco/ns#ActionInteraction
sco:ActionInteraction rdf:type owl:Class ;
                      rdfs:subClassOf sco:ServiceInteraction ;
                      rdfs:comment "A action that is triggered whenever a service capability from the device is triggered. A action is a method to mainpultae or trigger a process." ;
                      rdfs:label "Action Interaction" .


###  http://purl.org/sco/ns#DataModel
sco:DataModel rdf:type owl:Class ;
              rdfs:comment "The Data Model describes how data for a specific Service Capability for the exchange between the device and another device is prepared." ;
              rdfs:label "Data Model" .


###  http://purl.org/sco/ns#Device
sco:Device rdf:type owl:Class ;
           rdfs:comment "A device, capable of machine-to-machine (M2M) communication." ;
           rdfs:label "Device" .


###  http://purl.org/sco/ns#Format
sco:Format rdf:type owl:Class ;
           rdfs:comment "A kind of dataformat to interpret the data exchanged by the Service capability." ;
           rdfs:label "Format" .


###  http://purl.org/sco/ns#ProtocolStack
sco:ProtocolStack rdf:type owl:Class ;
                  rdfs:comment "The machine-to-machine communication protocol used to exchange information between two devices." ;
                  rdfs:label "Protocolstack" .


###  http://purl.org/sco/ns#ReadInteraction
sco:ReadInteraction rdf:type owl:Class ;
                    rdfs:subClassOf sco:ServiceInteraction ;
                    rdfs:comment "A reading of some data from the device whenever a service capability is triggered." ;
                    rdfs:label "Read Interaction" .


###  http://purl.org/sco/ns#ServiceCapability
sco:ServiceCapability rdf:type owl:Class ;
                      rdfs:comment "A service provided by a device to achieve some kind of processing. The service has often in machine-to-machine communication protocols other names, such as Characteristic in Bluetooth LE, Command or Attribute in ZigBee." ;
                      rdfs:label "Service Capability" .


###  http://purl.org/sco/ns#ServiceInteraction
sco:ServiceInteraction rdf:type owl:Class ;
                       rdfs:comment "A kind of interaction provided through the service capability from the device." ;
                       rdfs:label "Service Interaction" .


###  http://purl.org/sco/ns#SubscribeInteraction
sco:SubscribeInteraction rdf:type owl:Class ;
                         rdfs:subClassOf sco:ServiceInteraction ;
                         rdfs:comment "A subscribing to a service capability that is triggered when a change occurs to some data associated to the service capability." ;
                         rdfs:label "Subscribe Interaction" .


###  http://purl.org/sco/ns#TransformationRule
sco:TransformationRule rdf:type owl:Class ;
                       rdfs:comment "A custom transformation rule expressed with a kind of model ontology, such as Function Ontology, Binary Data Ontology, or OpenMath, that can be used to describe the necessary transformations for a payload." ;
                       rdfs:label "Transformation Rule" .


###  http://purl.org/sco/ns#WriteInteraction
sco:WriteInteraction rdf:type owl:Class ;
                     rdfs:subClassOf sco:ServiceInteraction ;
                     rdfs:comment "A writing of some data to the device whenever a service capability is triggered." ;
                     rdfs:label "Write Interaction" .


#################################################################
#    Individuals
#################################################################

###  http://purl.org/sco/ns#ArraySchema
sco:ArraySchema rdf:type owl:NamedIndividual ,
                         sco:Format .


###  http://purl.org/sco/ns#BluetoothLE
sco:BluetoothLE rdf:type owl:NamedIndividual ,
                         sco:ProtocolStack .


###  http://purl.org/sco/ns#Zigbee
sco:Zigbee rdf:type owl:NamedIndividual ,
                    sco:ProtocolStack .


###  https://www.w3.org/2019/wot/json-schema#BooleanSchema
<https://www.w3.org/2019/wot/json-schema#BooleanSchema> rdf:type owl:NamedIndividual ,
                                                                 sco:Format .


###  https://www.w3.org/2019/wot/json-schema#IntegerSchema
<https://www.w3.org/2019/wot/json-schema#IntegerSchema> rdf:type owl:NamedIndividual ,
                                                                 sco:Format .


###  https://www.w3.org/2019/wot/json-schema#NullSchema
<https://www.w3.org/2019/wot/json-schema#NullSchema> rdf:type owl:NamedIndividual ,
                                                              sco:Format .


###  https://www.w3.org/2019/wot/json-schema#NumberSchema
<https://www.w3.org/2019/wot/json-schema#NumberSchema> rdf:type owl:NamedIndividual ,
                                                                sco:Format .


###  https://www.w3.org/2019/wot/json-schema#ObjectSchema
<https://www.w3.org/2019/wot/json-schema#ObjectSchema> rdf:type owl:NamedIndividual ,
                                                                sco:Format .


###  https://www.w3.org/2019/wot/json-schema#StringSchema
<https://www.w3.org/2019/wot/json-schema#StringSchema> rdf:type owl:NamedIndividual ,
                                                                sco:Format .


[ schema:affiliation [ foaf:homepage <https://www.scs.fraunhofer.de/de/ueber-uns/organisation/data-spaces-and-iot-solutions.html> ;
                       foaf:name "Data Spaces and IoT Solutions"
                     ] ;
  rdfs:seeAlso <https://renedorsch.solidweb.org/#me> ;
  foaf:homepage <https://orcid.org/0000-0001-6857-7314> ;
  foaf:name "Rene Dorsch"
] .

[ schema:affiliation [ foaf:homepage <https://www.scs.fraunhofer.de/de/ueber-uns/organisation/data-spaces-and-iot-solutions.html> ;
                        foaf:name "Data Spaces and IoT Solutions"
                      ] ;
   rdfs:seeAlso <https://renedorsch.solidweb.org/#me> ;
   foaf:homepage <https://orcid.org/0000-0001-6857-7314> ;
   foaf:name "Rene Dorsch"
 ] .

[ schema:affiliation [ foaf:homepage <https://www.scs.fraunhofer.de/de/ueber-uns/organisation/data-spaces-and-iot-solutions.html> ;
                        foaf:name "Data Spaces and IoT Solutions"
                      ] ;
   rdfs:seeAlso <https://renedorsch.solidweb.org/#me> ;
   foaf:homepage <https://orcid.org/0000-0001-6857-7314> ;
   foaf:name "Rene Dorsch"
 ] .

[ schema:affiliation [ foaf:homepage <https://www.scs.fraunhofer.de/de/ueber-uns/organisation/data-spaces-and-iot-solutions.html> ;
                        foaf:name "Data Spaces and IoT Solutions"
                      ] ;
   rdfs:seeAlso <https://renedorsch.solidweb.org/#me> ;
   foaf:homepage <https://orcid.org/0000-0001-6857-7314> ;
   foaf:name "Rene Dorsch"
 ] .

[ schema:affiliation [ foaf:homepage <https://www.scs.fraunhofer.de/de/ueber-uns/organisation/data-spaces-and-iot-solutions.html> ;
                        foaf:name "Data Spaces and IoT Solutions"
                      ] ;
   rdfs:seeAlso <https://renedorsch.solidweb.org/#me> ;
   foaf:homepage <https://orcid.org/0000-0001-6857-7314> ;
   foaf:name "Rene Dorsch"
 ] .

#################################################################
#    Annotations
#################################################################

sco:hasManufacturer rdfs:label "has Manufacturer" ;
                     rdfs:comment "A organization that designed the device or its capabilitiy." .


#################################################################
#    General axioms
#################################################################

[ rdf:type owl:AllDisjointClasses ;
  owl:members ( sco:DataModel
                sco:Device
                sco:Format
                sco:ProtocolStack
                sco:ServiceCapability
                sco:ServiceInteraction
                sco:TransformationRule
              )
] .


###  Generated by the OWL API (version 4.5.9.2019-02-01T07:24:44Z) https://github.com/owlcs/owlapi
